theories/properties.v
@@ -1,0 +1,35 @@
+Set Implicit Arguments.
+Unset Strict Implicit.
+
+Require Import List.
+Import ListNotations.
+
+Require Import syntax semantics.
+
+Definition deliver_exists (ini : config) (target : name) (msg : message) :=
+  exists global_queue actions queue number actors_l actors_r,
+    let c := (conf (send_message target msg :: global_queue)
+              (actors_l
+                 ++ actor_state target actions queue number
+                 :: actors_r)) in
+    ini ~>* c /\ (exists c', c ~(Deliver)~> c').
+
+Definition open_exists (ini : config) (target : name) (msg : message) :=
+  exists global_queue behv queue number actors_l actors_r,
+    forall c,
+    c = (conf global_queue
+              (actors_l
+                 ++ actor_state target (become behv) (msg :: queue) number
+                 :: actors_r)) ->
+    ini ~>* c /\ (exists c', c ~(Open)~> c').
+
+Definition open_exists_with_behv (ini : config) (target : name) (msg : message) (behv : behavior) :=
+  exists global_queue queue number actors_l actors_r,
+    forall c,
+    c = (conf global_queue
+              (actors_l
+                 ++ actor_state target (become behv) (msg :: queue) number
+                 :: actors_r)) ->
+    ini ~>* c /\ (exists c', c ~(Open)~> c').
+
+(* (msg : message) じゃなくて (P : msg -> Prop) とかのほうが良さそう *)
